Prove sys_putc satisfies its dry spec

progs/io_os_connection.v
@@ -242,14 +242,6 @@ Local Open Scope Z.
 Definition getchar_pre' (m : mem) (witness : int -> IO_itree) (z : IO_itree) :=
   let k := witness in trace_incl (r <- read;; k r) z.
 
-(* getchar_pre' really is weaker. *)
-Goal forall m w z,
-  getchar_pre m w z -> getchar_pre' m w z.
-Proof.
-  unfold getchar_pre, getchar_pre'; intros ? *.
-  apply sutt_trace_incl.
-Qed.
-
 (* CertiKOS specs must terminate. Could get blocking version back by
    wrapping getchar in a loop. *)
 Definition getchar_post' (m0 m : mem) r (witness : (int -> IO_itree) * IO_itree) (z : IO_itree) :=
@@ -257,7 +249,7 @@ Definition getchar_post' (m0 m : mem) r (witness : (int -> IO_itree) * IO_itree)
     (* Success *)
     ((0 <= Int.signed r <= two_p 8 - 1 /\ let (k, _) := witness in z = k r) \/
     (* No character to read *)
-    let (_, z0) := witness in z = z0 /\ Int.signed r = -1).
+    (Int.signed r = -1 /\ let (_, z0) := witness in z = z0)).
 
 (** Traces *)
 Definition ostrace := list IOEvent.
@@ -268,14 +260,18 @@ Definition IOEvent_eq (e1 e2 : IOEvent) : {e1 = e2} + {e1 <> e2} :=
 Definition trace_event_rtype (e : IOEvent) :=
   match e with
   | IOEvRecv _ _ _ => void
+  | IOEvSend _ _ => void
   | IOEvGetc _ _ _ => int
+  | IOEvPutc _ _ => unit
   end.
 
 Definition io_event_of_io_tevent (e : IOEvent)
   : option (IO_event (trace_event_rtype e) * (trace_event_rtype e)) :=
   match e with
   | IOEvRecv _ _ _ => None
+  | IOEvSend _ _ => None
   | IOEvGetc _ _ r => Some (ERead, Int.repr r)
+  | IOEvPutc _ r => Some (EWrite (Int.repr r), tt)
   end.
 
 Fixpoint trace_of_ostrace (t : ostrace) : @trace IO_event unit :=
@@ -287,41 +283,6 @@ Fixpoint trace_of_ostrace (t : ostrace) : @trace IO_event unit :=
       | _ => trace_of_ostrace t'
       end
   end.
-
-Section SanityChecks.
-  Variable k : int -> itree IO_event unit.
-  Definition tree := (r <- read;; k r).
-
-  Goal is_trace tree (@TEnd _ unit).
-  Proof.
-    hnf; cbn.
-    constructor.
-  Qed.
-
-  Goal is_trace tree (@TEventEnd _ unit _ ERead).
-  Proof.
-    hnf; cbn.
-    constructor.
-  Qed.
-
-  Goal is_trace tree (@TEventResponse _ unit _ ERead Int.zero TEnd).
-  Proof.
-    hnf; cbn.
-    repeat constructor.
-  Qed.
-
-  Goal is_trace tree (trace_of_ostrace nil).
-  Proof.
-    hnf; cbn.
-    constructor.
-  Qed.
-
-  Goal is_trace tree (trace_of_ostrace (IOEvGetc 0 O 0 :: IOEvRecv 0 O 0 :: nil)).
-  Proof.
-    hnf; cbn.
-    repeat constructor.
-  Qed.
-End SanityChecks.
 
 (** Trace Invariants *)
 Section Invariants.
@@ -336,6 +297,7 @@ Section Invariants.
         let cons' := if Zlength cons <? CONS_BUFFER_MAX_CHARS then cons else tl cons in
         cons' ++ (c, logIdx, strIdx) :: nil
       | IOEvGetc _ _ _ => tl cons
+      | _ => cons
       end
     end.
   Definition compute_console tr := compute_console' (rev tr).
@@ -370,11 +332,11 @@ Section Invariants.
 
   (* All trace invariants hold. *)
   Record valid_trace (st : RData) := {
-    vt_trace_serial : valid_trace_serial st.(io_log) st.(com1).(l1);
-    vt_trace_ordered : valid_trace_ordered st.(io_log);
-    vt_trace_user : valid_trace_user st.(io_log);
-    vt_trace_unique : valid_trace_unique st.(io_log);
-    vt_trace_console : valid_trace_console st.(io_log) st.(console).(cons_buf);
+    vt_trace_serial : valid_trace_serial st.(io_rx_log) st.(com1).(l1);
+    vt_trace_ordered : valid_trace_ordered st.(io_rx_log);
+    vt_trace_user : valid_trace_user st.(io_rx_log);
+    vt_trace_unique : valid_trace_unique st.(io_rx_log);
+    vt_trace_console : valid_trace_console st.(io_rx_log) st.(console).(cons_buf);
   }.
 
   (* Console entries are ordered by logIdx and strIdx *)
@@ -426,7 +388,8 @@ Section Invariants.
   Proof.
     induction tr as [| ev tr]; cbn; intros * Hcons;
       [contradict Hcons; auto using app_cons_not_nil |].
-    destruct ev; cbn in Hcons.
+    destruct ev; cbn in Hcons;
+      try solve [edestruct IHtr as (? & ? & ? & ?); eauto; subst; eauto using app_comm_cons].
     - rewrite app_comm_cons, app_assoc in Hcons.
       destruct @app_tail_case with (1 := Hcons) as [(? & ? & Hcons') | (? & Hcons' & ?)]; inj; subst;
         destruct (_ <? _).
@@ -483,7 +446,8 @@ Section Invariants.
     end.
   Proof.
     unfold lex_le, lex_lt; intros * Horder Hcons Hcons'.
-    destruct ev; cbn in Hcons'.
+    destruct ev; cbn in Hcons';
+      try solve [rewrite Hcons in Hcons'; inj; auto].
     - destruct (_ <? _).
       + erewrite hd_error_app in Hcons'; eauto; inj; auto.
       + destruct (hd_error_app_case (tl (compute_console' tr)) (c0, logIdx0, strIdx0)) as [Heq | Heq];
@@ -983,12 +947,14 @@ Section Invariants.
     - eapply IHn; [| eauto].
       destruct st; inv Hvalid; constructor; cbn in *; auto.
       destruct com1; cbn in *; red; intros; subst; edestruct vt_trace_serial0; eauto.
-      split; auto; lia.
+      prename serial_intr into Hspec'; unfold serial_intr in Hspec'; destruct_spec Hspec'.
+      cbn; split; auto; lia.
     - eapply IHn; [| eauto].
       eapply cons_intr_aux_preserve_valid_trace; [| eauto].
       destruct st; inv Hvalid; constructor; cbn in *; auto.
       destruct com1; cbn in *; red; intros; subst; edestruct vt_trace_serial0; eauto.
-      split; auto; lia.
+      prename serial_intr into Hspec'; unfold serial_intr in Hspec'; destruct_spec Hspec'.
+      cbn; split; auto; lia.
   Qed.
 
   Lemma serial_intr_disable_preserve_valid_trace : forall st st',
@@ -1039,9 +1005,9 @@ Section Invariants.
     destruct st; inv Hvalid; constructor; cbn in *; auto.
   Qed.
 
-  Lemma serial_putc_preserve_valid_trace : forall st c st',
+  Lemma serial_putc_preserve_valid_trace : forall st c st' r,
     valid_trace st ->
-    serial_putc_spec c st = Some st' ->
+    serial_putc_spec c st = Some (st', r) ->
     valid_trace st'.
   Proof.
     unfold serial_putc_spec; intros * Hvalid Hspec; destruct_spec Hspec; eauto.
@@ -1101,9 +1067,9 @@ Section Invariants.
     eapply cons_buf_read_preserve_valid_trace; eauto.
   Qed.
 
-  Lemma thread_serial_putc_preserve_valid_trace : forall st c st',
+  Lemma thread_serial_putc_preserve_valid_trace : forall st c st' r,
     valid_trace st ->
-    thread_serial_putc_spec c st = Some st' ->
+    thread_serial_putc_spec c st = Some (st', r) ->
     valid_trace st'.
   Proof.
     unfold thread_serial_putc_spec; intros * Hvalid Hspec; destruct_spec Hspec.
@@ -1131,6 +1097,7 @@ Section Invariants.
   Proof.
     unfold sys_putc_spec; intros * Hvalid Hspec; destruct_spec Hspec.
     eapply uctx_set_errno_preserve_valid_trace; [| eauto].
+    eapply uctx_set_retval1_preserve_valid_trace; [| eauto].
     eapply thread_serial_intr_enable_preserve_valid_trace; [| eauto].
     eapply thread_serial_putc_preserve_valid_trace; [| eauto].
     eapply thread_serial_intr_disable_preserve_valid_trace; [| eauto].
@@ -1138,7 +1105,7 @@ Section Invariants.
   Qed.
 
   (** At most one user-visible event is generated. *)
-  Definition trace_case t t' ret :=
+  Definition getc_trace_case t t' ret :=
     let new := trace_of_ostrace (strip_common_prefix IOEvent_eq t t') in
     t = common_prefix IOEvent_eq t t' /\
     ((ret = -1 /\ new = trace_of_ostrace nil) \/
@@ -1152,7 +1119,7 @@ Section Invariants.
   Proof.
     induction otr as [| ev otr]; cbn; intros *; auto.
     destruct ev; cbn; auto.
-    rewrite IHotr; auto.
+    all: rewrite IHotr; auto.
   Qed.
 
   Lemma IOEvRecvs_not_visible : forall tr,
@@ -1171,18 +1138,18 @@ Section Invariants.
     destruct Hin as (? & ? & ? & ? & ?); eauto.
   Qed.
 
-  Lemma trace_case_refl : forall st, trace_case st st (-1).
+  Lemma getc_trace_case_refl : forall st, getc_trace_case st st (-1).
   Proof.
     red; intros; unfold strip_common_prefix.
     rewrite common_prefix_full, leb_correct, skipn_exact_length; cbn; auto.
   Qed.
 
-  Local Hint Resolve trace_case_refl.
+  Local Hint Resolve getc_trace_case_refl.
 
-  Lemma trace_case_trans : forall t t' t'' r,
-    trace_case t t' (-1) ->
-    trace_case t' t'' r ->
-    trace_case t t'' r.
+  Lemma getc_trace_case_trans : forall t t' t'' r,
+    getc_trace_case t t' (-1) ->
+    getc_trace_case t' t'' r ->
+    getc_trace_case t t'' r.
   Proof.
     intros * Htr Htr'; red.
     destruct Htr as (Heq & Htr), Htr' as (Heq' & Htr'); subst.
@@ -1197,10 +1164,10 @@ Section Invariants.
     destruct Htr as [(? & ->) | ?], Htr' as [(? & ->) | ?]; subst; auto; easy.
   Qed.
 
-  Lemma trace_case_trans' : forall t t' t'' r,
-    trace_case t t' r ->
-    trace_case t' t'' (-1) ->
-    trace_case t t'' r.
+  Lemma getc_trace_case_trans' : forall t t' t'' r,
+    getc_trace_case t t' r ->
+    getc_trace_case t' t'' (-1) ->
+    getc_trace_case t t'' r.
   Proof.
     intros * Htr Htr'; red.
     destruct Htr as (Heq & Htr), Htr' as (Heq' & Htr'); subst.
@@ -1216,11 +1183,11 @@ Section Invariants.
     rewrite Heq; cbn; auto; constructor.
   Qed.
 
-  Lemma cons_intr_aux_trace_case : forall st st',
+  Lemma cons_intr_aux_getc_trace_case : forall st st',
     cons_intr_aux st = Some st' ->
-    trace_case st.(io_log) st'.(io_log) (-1).
+    getc_trace_case st.(io_rx_log) st'.(io_rx_log) (-1).
   Proof.
-    unfold cons_intr_aux, trace_case; intros * Hspec; destruct_spec Hspec.
+    unfold cons_intr_aux, getc_trace_case; intros * Hspec; destruct_spec Hspec.
     - prename (Coqlib.zeq _ _ = _) into Htmp; clear Htmp.
       destruct st; cbn in *; subst; cbn in *.
       rewrite common_prefix_app, app_length, leb_correct by lia.
@@ -1231,106 +1198,98 @@ Section Invariants.
       rewrite skipn_app1, skipn_exact_length; cbn; auto using mkRecvEvents_not_visible.
   Qed.
 
-  Lemma serial_intr_enable_aux_trace_case : forall n st st',
+  Lemma serial_intr_enable_aux_getc_trace_case : forall n st st',
     serial_intr_enable_aux n st = Some st' ->
-    trace_case st.(io_log) st'.(io_log) (-1).
+    getc_trace_case st.(io_rx_log) st'.(io_rx_log) (-1).
   Proof.
     induction n; intros * Hspec; cbn -[cons_intr_aux] in Hspec; inj; auto.
     destruct_spec Hspec; auto.
     prename cons_intr_aux into Hspec'.
-    eapply trace_case_trans; [eapply cons_intr_aux_trace_case |]; eauto.
+    eapply getc_trace_case_trans; [eapply cons_intr_aux_getc_trace_case |]; eauto.
   Qed.
 
-  Lemma serial_intr_enable_trace_case : forall st st',
+  Lemma serial_intr_enable_getc_trace_case : forall st st',
     serial_intr_enable_spec st = Some st' ->
-    trace_case st.(io_log) st'.(io_log) (-1).
+    getc_trace_case st.(io_rx_log) st'.(io_rx_log) (-1).
   Proof.
     unfold serial_intr_enable_spec; intros * Hspec; destruct_spec Hspec.
     prename serial_intr_enable_aux into Hspec.
-    eapply serial_intr_enable_aux_trace_case in Hspec.
+    eapply serial_intr_enable_aux_getc_trace_case in Hspec.
     destruct st, r; auto.
   Qed.
 
-  Lemma serial_intr_disable_aux_trace_case : forall n mask st st',
+  Lemma serial_intr_disable_aux_getc_trace_case : forall n mask st st',
     serial_intr_disable_aux n mask st = Some st' ->
-    trace_case st.(io_log) st'.(io_log) (-1).
+    getc_trace_case st.(io_rx_log) st'.(io_rx_log) (-1).
   Proof.
     induction n; intros * Hspec; cbn -[cons_intr_aux] in Hspec; inj; auto.
     destruct_spec Hspec; auto.
     - eapply IHn in Hspec.
       destruct st; auto.
     - prename cons_intr_aux into Hspec'.
-      eapply cons_intr_aux_trace_case in Hspec'.
+      eapply cons_intr_aux_getc_trace_case in Hspec'.
       eapply IHn in Hspec.
-      eapply trace_case_trans; [| eapply Hspec]; eauto.
+      eapply getc_trace_case_trans; [| eapply Hspec]; eauto.
       destruct st; auto.
   Qed.
 
-  Lemma serial_intr_disable_trace_case : forall st st',
+  Lemma serial_intr_disable_getc_trace_case : forall st st',
     serial_intr_disable_spec st = Some st' ->
-    trace_case st.(io_log) st'.(io_log) (-1).
+    getc_trace_case st.(io_rx_log) st'.(io_rx_log) (-1).
   Proof.
     unfold serial_intr_disable_spec; intros * Hspec; destruct_spec Hspec.
     prename serial_intr_disable_aux into Hspec.
-    eapply serial_intr_disable_aux_trace_case in Hspec.
+    eapply serial_intr_disable_aux_getc_trace_case in Hspec.
     destruct st, r; auto.
   Qed.
 
-  Lemma thread_serial_intr_enable_trace_case : forall st st',
+  Lemma thread_serial_intr_enable_getc_trace_case : forall st st',
     thread_serial_intr_enable_spec st = Some st' ->
-    trace_case st.(io_log) st'.(io_log) (-1).
+    getc_trace_case st.(io_rx_log) st'.(io_rx_log) (-1).
   Proof.
     unfold thread_serial_intr_enable_spec; intros * Hspec; destruct_spec Hspec.
-    eapply serial_intr_enable_trace_case; eauto.
+    eapply serial_intr_enable_getc_trace_case; eauto.
   Qed.
 
-  Lemma thread_serial_intr_disable_trace_case : forall st st',
+  Lemma thread_serial_intr_disable_getc_trace_case : forall st st',
     thread_serial_intr_disable_spec st = Some st' ->
-    trace_case st.(io_log) st'.(io_log) (-1).
+    getc_trace_case st.(io_rx_log) st'.(io_rx_log) (-1).
   Proof.
     unfold thread_serial_intr_disable_spec; intros * Hspec; destruct_spec Hspec.
-    eapply serial_intr_disable_trace_case; eauto.
+    eapply serial_intr_disable_getc_trace_case; eauto.
   Qed.
 
-  Lemma uctx_set_retval1_trace_case : forall st v st',
+  Lemma uctx_set_retval1_getc_trace_case : forall st v st',
     uctx_set_retval1_spec v st = Some st' ->
-    trace_case st.(io_log) st'.(io_log) (-1).
+    getc_trace_case st.(io_rx_log) st'.(io_rx_log) (-1).
   Proof.
     unfold uctx_set_retval1_spec; intros * Hspec; destruct_spec Hspec.
     destruct st; auto.
   Qed.
 
-  Lemma uctx_set_errno_trace_case : forall st e st',
+  Lemma uctx_set_errno_getc_trace_case : forall st e st',
     uctx_set_errno_spec e st = Some st' ->
-    trace_case st.(io_log) st'.(io_log) (-1).
+    getc_trace_case st.(io_rx_log) st'.(io_rx_log) (-1).
   Proof.
     unfold uctx_set_errno_spec; intros * Hspec; destruct_spec Hspec.
     destruct st; auto.
   Qed.
 
-  Lemma serial_putc_trace_case : forall st c st',
-    serial_putc_spec c st = Some st' ->
-    trace_case st.(io_log) st'.(io_log) (-1).
-  Proof.
-    unfold serial_putc_spec; intros * Hspec; destruct_spec Hspec; eauto.
-    all: destruct st; auto.
-  Qed.
-
-  Lemma cons_buf_read_trace_case : forall st st' c,
+  Lemma cons_buf_read_getc_trace_case : forall st st' c,
     valid_trace st ->
     cons_buf_read_spec st = Some (st', c) ->
-    trace_case st.(io_log) st'.(io_log) c /\ -1 <= c <= 255.
+    getc_trace_case st.(io_rx_log) st'.(io_rx_log) c /\ -1 <= c <= 255.
   Proof.
     unfold cons_buf_read_spec; intros * Hvalid Hspec; destruct_spec Hspec.
     { split; eauto; lia. }
     prename (cons_buf _ = _) into Hcons.
-    destruct st; cbn in *; unfold trace_case.
+    destruct st; cbn in *; unfold getc_trace_case.
     unfold strip_common_prefix.
     rewrite common_prefix_app, app_length, leb_correct by lia.
     rewrite skipn_app1, skipn_exact_length; cbn; auto.
     inv Hvalid; cbn in *.
     rewrite vt_trace_console0 in Hcons.
-    assert (Hin: In (c, z0, n) (compute_console io_log)) by (rewrite Hcons; cbn; auto).
+    assert (Hin: In (c, z0, n) (compute_console io_rx_log)) by (rewrite Hcons; cbn; auto).
     apply in_console_in_trace in Hin.
     apply in_split in Hin; destruct Hin as (? & ? & ?); subst.
     edestruct vt_trace_serial0 as (_ & Henv); eauto.
@@ -1342,21 +1301,13 @@ Section Invariants.
     split; auto; lia.
   Qed.
 
-  Lemma thread_cons_buf_read_trace_case : forall st st' c,
+  Lemma thread_cons_buf_read_getc_trace_case : forall st st' c,
     valid_trace st ->
     thread_cons_buf_read_spec st = Some (st', c) ->
-    trace_case st.(io_log) st'.(io_log) c /\ -1 <= c <= 255.
+    getc_trace_case st.(io_rx_log) st'.(io_rx_log) c /\ -1 <= c <= 255.
   Proof.
     unfold thread_cons_buf_read_spec; intros * Hvalid Hspec; destruct_spec Hspec.
-    eapply cons_buf_read_trace_case; eauto.
-  Qed.
-
-  Lemma thread_serial_putc_trace_case : forall st c st',
-    thread_serial_putc_spec c st = Some st' ->
-    trace_case st.(io_log) st'.(io_log) (-1).
-  Proof.
-    unfold thread_serial_putc_spec; intros * Hspec; destruct_spec Hspec.
-    eapply serial_putc_trace_case; eauto.
+    eapply cons_buf_read_getc_trace_case; eauto.
   Qed.
 
   Definition get_sys_ret (st : RData) :=
@@ -1367,7 +1318,7 @@ Section Invariants.
     valid_trace st ->
     sys_getc_spec st = Some st' ->
     get_sys_ret st' = Vint ret ->
-    trace_case st.(io_log) st'.(io_log) (Int.signed ret).
+    getc_trace_case st.(io_rx_log) st'.(io_rx_log) (Int.signed ret).
   Proof.
     unfold sys_getc_spec, get_sys_ret; intros * Hvalid Hspec Hret; destruct_spec Hspec.
     prename thread_serial_intr_disable_spec into Hspec1.
@@ -1379,15 +1330,15 @@ Section Invariants.
     assert (valid_trace r1) by eauto using thread_serial_intr_enable_preserve_valid_trace.
     assert (valid_trace r2) by eauto using uctx_set_retval1_preserve_valid_trace.
     assert (valid_trace st') by eauto using uctx_set_errno_preserve_valid_trace.
-    eapply thread_serial_intr_disable_trace_case in Hspec1 as Htr.
-    eapply thread_cons_buf_read_trace_case in Hspec2 as (Htr1 & Hrange); auto.
-    eapply thread_serial_intr_enable_trace_case in Hspec3 as Htr2.
-    eapply uctx_set_retval1_trace_case in Hspec4 as Htr3.
-    eapply uctx_set_errno_trace_case in Hspec as Htr4.
-    eapply trace_case_trans'; [| eapply Htr4].
-    eapply trace_case_trans'; [| eapply Htr3].
-    eapply trace_case_trans'; [| eapply Htr2].
-    eapply trace_case_trans; [eapply Htr |]; eauto.
+    eapply thread_serial_intr_disable_getc_trace_case in Hspec1 as Htr.
+    eapply thread_cons_buf_read_getc_trace_case in Hspec2 as (Htr1 & Hrange); auto.
+    eapply thread_serial_intr_enable_getc_trace_case in Hspec3 as Htr2.
+    eapply uctx_set_retval1_getc_trace_case in Hspec4 as Htr3.
+    eapply uctx_set_errno_getc_trace_case in Hspec as Htr4.
+    eapply getc_trace_case_trans'; [| eapply Htr4].
+    eapply getc_trace_case_trans'; [| eapply Htr3].
+    eapply getc_trace_case_trans'; [| eapply Htr2].
+    eapply getc_trace_case_trans; [eapply Htr |]; eauto.
     enough (z = Int.signed ret); subst; auto.
     clear -Hspec Hspec4 Hret Htr1 Hrange.
     unfold uctx_set_retval1_spec in Hspec4; destruct_spec Hspec4.
@@ -1395,6 +1346,237 @@ Section Invariants.
     destruct r1; cbn in *; subst.
     repeat (rewrite ZMap.gss in Hret || rewrite ZMap.gso in Hret by easy); inj.
     rewrite Int.signed_repr; auto; cbn; lia.
+  Qed.
+
+  Definition putc_trace_case t t' c ret :=
+    let new := trace_of_ostrace (strip_common_prefix IOEvent_eq t t') in
+    t = common_prefix IOEvent_eq t t' /\
+    ((ret = -1 /\ new = trace_of_ostrace nil) \/
+     (ret = c mod 256 /\ forall logIdx,
+        new = trace_of_ostrace (IOEvPutc logIdx c :: nil))).
+
+  Lemma putc_trace_case_refl : forall st c, putc_trace_case st st c (-1).
+  Proof.
+    red; intros; unfold strip_common_prefix.
+    rewrite common_prefix_full, leb_correct, skipn_exact_length; cbn; auto.
+  Qed.
+
+  Local Hint Resolve putc_trace_case_refl.
+
+  Lemma putc_trace_case_trans : forall t t' t'' c r,
+    putc_trace_case t t' c (-1) ->
+    putc_trace_case t' t'' c r ->
+    putc_trace_case t t'' c r.
+  Proof.
+    intros * Htr Htr'; red.
+    destruct Htr as (Heq & Htr), Htr' as (Heq' & Htr'); subst.
+    apply common_prefix_correct in Heq; apply common_prefix_correct in Heq'.
+    destruct Heq, Heq'; subst.
+    unfold strip_common_prefix in *.
+    rewrite !app_length, leb_correct in * by lia.
+    rewrite <- app_assoc.
+    rewrite common_prefix_app, skipn_app1, skipn_exact_length in *;
+      rewrite ?app_length; auto; cbn in *.
+    rewrite trace_of_ostrace_app.
+    pose proof (Z.mod_pos_bound c 256 ltac:(lia)).
+    destruct Htr as [(? & ->) | (? & ?)], Htr' as [(? & ->) | ?]; subst; auto; exfalso; lia.
+  Qed.
+
+  Lemma putc_trace_case_trans' : forall t t' t'' c r,
+    putc_trace_case t t' c r ->
+    putc_trace_case t' t'' c (-1) ->
+    putc_trace_case t t'' c r.
+  Proof.
+    intros * Htr Htr'; red.
+    destruct Htr as (Heq & Htr), Htr' as (Heq' & Htr'); subst.
+    apply common_prefix_correct in Heq; apply common_prefix_correct in Heq'.
+    destruct Heq, Heq'; subst.
+    unfold strip_common_prefix in *.
+    rewrite !app_length, leb_correct in * by lia.
+    rewrite <- app_assoc.
+    rewrite common_prefix_app, skipn_app1, skipn_exact_length in *;
+      rewrite ?app_length; auto; cbn in *.
+    rewrite trace_of_ostrace_app.
+    pose proof (Z.mod_pos_bound c 256 ltac:(lia)).
+    destruct Htr as [(? & ->) | (? & Heq)], Htr' as [(? & ->) | (? & ?)]; subst; auto; try easy.
+    rewrite Heq; cbn; auto; constructor.
+    exfalso; lia.
+  Qed.
+
+  Lemma cons_intr_aux_putc_trace_case : forall st st' c,
+    cons_intr_aux st = Some st' ->
+    putc_trace_case st.(io_tx_log) st'.(io_tx_log) c (-1).
+  Proof.
+    unfold cons_intr_aux, putc_trace_case; intros * Hspec; destruct_spec Hspec.
+    - prename (Coqlib.zeq _ _ = _) into Htmp; clear Htmp.
+      destruct st; cbn in *; subst; cbn in *.
+      rewrite common_prefix_full, leb_correct, skipn_exact_length by lia; auto.
+    - prename (Coqlib.zeq _ _ = _) into Htmp; clear Htmp.
+      destruct st; cbn in *; subst; cbn in *.
+      rewrite common_prefix_full, leb_correct, skipn_exact_length by lia; auto.
+  Qed.
+
+  Lemma serial_intr_enable_aux_putc_trace_case : forall n st st' c,
+    serial_intr_enable_aux n st = Some st' ->
+    putc_trace_case st.(io_tx_log) st'.(io_tx_log) c (-1).
+  Proof.
+    induction n; intros * Hspec; cbn -[cons_intr_aux] in Hspec; inj; auto.
+    destruct_spec Hspec; auto.
+    prename cons_intr_aux into Hspec'.
+    eapply putc_trace_case_trans; [eapply cons_intr_aux_putc_trace_case |]; eauto.
+  Qed.
+
+  Lemma serial_intr_enable_putc_trace_case : forall st st' c,
+    serial_intr_enable_spec st = Some st' ->
+    putc_trace_case st.(io_tx_log) st'.(io_tx_log) c (-1).
+  Proof.
+    unfold serial_intr_enable_spec; intros * Hspec; destruct_spec Hspec.
+    prename serial_intr_enable_aux into Hspec.
+    eapply serial_intr_enable_aux_putc_trace_case in Hspec.
+    destruct st, r; eauto.
+  Qed.
+
+  Lemma serial_intr_putc_trace_case : forall d d' tr,
+    serial_intr d = (d', tr) ->
+    trace_of_ostrace tr = TEnd.
+  Proof.
+    unfold serial_intr; intros * Hspec; destruct_spec Hspec.
+    destruct o; auto.
+  Qed.
+
+  Lemma serial_intr_disable_aux_putc_trace_case : forall n mask st st' c,
+    serial_intr_disable_aux n mask st = Some st' ->
+    putc_trace_case st.(io_tx_log) st'.(io_tx_log) c (-1).
+  Proof.
+    induction n; intros * Hspec; cbn -[cons_intr_aux] in Hspec; inj; auto.
+    destruct_spec Hspec; auto.
+    - eapply IHn in Hspec.
+      destruct st; cbn in *.
+      prename serial_intr into Hspec'.
+      unfold serial_intr in Hspec'; destruct_spec Hspec'.
+      destruct o; cbn in *.
+      + eapply putc_trace_case_trans; [| eauto].
+        red; unfold strip_common_prefix.
+        rewrite !app_length, leb_correct by lia.
+        rewrite common_prefix_app, skipn_app1, skipn_exact_length; auto.
+      + rewrite app_nil_r in Hspec; auto.
+    - prename cons_intr_aux into Hspec'.
+      eapply cons_intr_aux_putc_trace_case in Hspec'.
+      eapply IHn in Hspec.
+      eapply putc_trace_case_trans; [| eapply Hspec]; eauto.
+      destruct st; cbn in *.
+      prename serial_intr into Hspec''.
+      unfold serial_intr in Hspec''; destruct_spec Hspec''.
+      destruct o; cbn in *.
+      + eapply putc_trace_case_trans; [| eauto].
+        red; unfold strip_common_prefix.
+        rewrite !app_length, leb_correct by lia.
+        rewrite common_prefix_app, skipn_app1, skipn_exact_length; auto.
+      + rewrite app_nil_r in Hspec'; auto.
+  Qed.
+
+  Lemma serial_intr_disable_putc_trace_case : forall st st' c,
+    serial_intr_disable_spec st = Some st' ->
+    putc_trace_case st.(io_tx_log) st'.(io_tx_log) c (-1).
+  Proof.
+    unfold serial_intr_disable_spec; intros * Hspec; destruct_spec Hspec.
+    prename serial_intr_disable_aux into Hspec.
+    eapply serial_intr_disable_aux_putc_trace_case in Hspec.
+    destruct st, r; eauto.
+  Qed.
+
+  Lemma thread_serial_intr_enable_putc_trace_case : forall st st' c,
+    thread_serial_intr_enable_spec st = Some st' ->
+    putc_trace_case st.(io_tx_log) st'.(io_tx_log) c (-1).
+  Proof.
+    unfold thread_serial_intr_enable_spec; intros * Hspec; destruct_spec Hspec.
+    eapply serial_intr_enable_putc_trace_case; eauto.
+  Qed.
+
+  Lemma thread_serial_intr_disable_putc_trace_case : forall st st' c,
+    thread_serial_intr_disable_spec st = Some st' ->
+    putc_trace_case st.(io_tx_log) st'.(io_tx_log) c (-1).
+  Proof.
+    unfold thread_serial_intr_disable_spec; intros * Hspec; destruct_spec Hspec.
+    eapply serial_intr_disable_putc_trace_case; eauto.
+  Qed.
+
+  Lemma uctx_set_retval1_putc_trace_case : forall st v st' c,
+    uctx_set_retval1_spec v st = Some st' ->
+    putc_trace_case st.(io_tx_log) st'.(io_tx_log) c (-1).
+  Proof.
+    unfold uctx_set_retval1_spec; intros * Hspec; destruct_spec Hspec.
+    destruct st; auto.
+  Qed.
+
+  Lemma uctx_set_errno_putc_trace_case : forall st e st' c,
+    uctx_set_errno_spec e st = Some st' ->
+    putc_trace_case st.(io_tx_log) st'.(io_tx_log) c (-1).
+  Proof.
+    unfold uctx_set_errno_spec; intros * Hspec; destruct_spec Hspec.
+    destruct st; auto.
+  Qed.
+
+  Lemma serial_putc_putc_trace_case : forall st c st' r,
+    serial_putc_spec c st = Some (st', r) ->
+    putc_trace_case st.(io_tx_log) st'.(io_tx_log) c r.
+  Proof.
+    unfold serial_putc_spec; intros * Hspec; destruct_spec Hspec; eauto.
+    - prename (Coqlib.zeq _ _ = _) into Htmp; clear Htmp.
+      destruct st; cbn in *; subst; red.
+      unfold strip_common_prefix.
+      rewrite !app_length, leb_correct by lia.
+      rewrite common_prefix_app, skipn_app1, skipn_exact_length; auto.
+    - prename (Coqlib.zeq _ _ = _) into Htmp; clear Htmp.
+      destruct st; cbn in *; subst; red.
+      unfold strip_common_prefix.
+      rewrite !app_length, leb_correct by lia.
+      rewrite common_prefix_app, skipn_app1, skipn_exact_length; auto.
+  Qed.
+
+  Lemma thread_serial_putc_putc_trace_case : forall st c st' r,
+    thread_serial_putc_spec c st = Some (st', r) ->
+    putc_trace_case st.(io_tx_log) st'.(io_tx_log) c r.
+  Proof.
+    unfold thread_serial_putc_spec; intros * Hspec; destruct_spec Hspec.
+    eapply serial_putc_putc_trace_case; eauto.
+  Qed.
+
+  Definition get_sys_arg (st : RData) :=
+    let curid := ZMap.get st.(CPU_ID) st.(cid) in
+    ZMap.get U_EBX (ZMap.get curid st.(uctxt)).
+
+  Lemma sys_putc_trace_case : forall st st' c ret,
+    sys_putc_spec st = Some st' ->
+    get_sys_arg st = Vint c ->
+    get_sys_ret st' = Vint ret ->
+    putc_trace_case st.(io_tx_log) st'.(io_tx_log) (Int.unsigned c) (Int.signed ret).
+  Proof.
+    unfold sys_putc_spec, get_sys_arg, get_sys_ret; intros * Hspec Harg Hret; destruct_spec Hspec.
+    prename thread_serial_intr_disable_spec into Hspec1.
+    prename thread_serial_putc_spec into Hspec2.
+    prename thread_serial_intr_enable_spec into Hspec3.
+    prename uctx_set_retval1_spec into Hspec4.
+    prename uctx_arg2_spec into Hspec5.
+    eapply thread_serial_intr_disable_putc_trace_case in Hspec1 as Htr.
+    eapply thread_serial_putc_putc_trace_case in Hspec2 as (Htr1 & Hrange); auto.
+    eapply thread_serial_intr_enable_putc_trace_case in Hspec3 as Htr2.
+    eapply uctx_set_retval1_putc_trace_case in Hspec4 as Htr3.
+    eapply uctx_set_errno_putc_trace_case in Hspec as Htr4.
+    eapply putc_trace_case_trans'; [| eapply Htr4].
+    eapply putc_trace_case_trans'; [| eapply Htr3].
+    eapply putc_trace_case_trans'; [| eapply Htr2].
+    eapply putc_trace_case_trans; [eapply Htr |]; eauto.
+    enough (z0 = Int.signed ret /\ z = Int.unsigned c) as (? & ?); subst; [split; auto |].
+    clear -Hspec Hspec4 Hspec5 Harg Hret Htr1 Hrange.
+    unfold uctx_set_retval1_spec in Hspec4; destruct_spec Hspec4.
+    unfold uctx_set_errno_spec in Hspec; destruct_spec Hspec.
+    unfold uctx_arg2_spec in Hspec5; destruct_spec Hspec5.
+    destruct r1; cbn in *; subst.
+    repeat (rewrite ZMap.gss in Hret || rewrite ZMap.gso in Hret by easy); inj.
+    rewrite Int.signed_repr; auto; cbn; try lia.
+    pose proof (Z.mod_pos_bound (Int.unsigned c) 256 ltac:(lia)).
+    destruct Hrange as [(? & ?) | (? & ?)]; lia.
   Qed.
 
 End Invariants.
@@ -1415,17 +1597,17 @@ Section SpecsCorrect.
     consume_trace z0 z t.
 
   (* TODO: memory *)
-  Record sys_correct k z m st st' ret := {
+  Record R_sys_getc_correct k z m st st' ret := {
     (* New itree is old k applied to result, or same as old itree if nothing
        to read *)
-    z' := if 0 <=? Int.signed ret then k ret else z;
+    getc_z' := if 0 <=? Int.signed ret then k ret else z;
 
     (* Post condition holds on new state, itree, and result *)
-    post_ok : getchar_post' m m ret (k, z) z';
+    getc_post_ok : getchar_post' m m ret (k, z) getc_z';
     (* The itrees and OS traces agree on the external events *)
-    itree_trace_ok : trace_itree_match z z' st.(io_log) st'.(io_log);
+    getc_itree_trace_ok : trace_itree_match z getc_z' st.(io_rx_log) st'.(io_rx_log);
     (* The new trace is valid *)
-    trace_ok : valid_trace st';
+    getc_trace_ok : valid_trace st';
   }.
 
   Lemma sys_getc_correct k z m st st' :
@@ -1437,14 +1619,14 @@ Section SpecsCorrect.
     sys_getc_spec st = Some st' ->
     exists ret,
       get_sys_ret st' = Vint ret /\
-      sys_correct k z m st st' ret.
+      R_sys_getc_correct k z m st st' ret.
   Proof.
     unfold getchar_pre', get_sys_ret; intros Hvalid Hpre Hspec.
     apply sys_getc_preserve_valid_trace in Hspec as Hvalid'; auto.
     pose proof Hspec as Htrace_case.
     unfold sys_getc_spec in Hspec; destruct_spec Hspec.
     prename (thread_cons_buf_read_spec) into Hread.
-    apply thread_cons_buf_read_trace_case in Hread as (_ & ?).
+    apply thread_cons_buf_read_getc_trace_case in Hread as (_ & ?).
     2: eapply (thread_serial_intr_disable_preserve_valid_trace st); eauto.
     unfold uctx_set_errno_spec in Hspec; destruct_spec Hspec.
     prename (uctx_set_retval1_spec) into Hspec.
@@ -1469,6 +1651,72 @@ Section SpecsCorrect.
       rewrite Zle_imp_le_bool in Htrace by lia.
       unshelve erewrite Heq; try solve [constructor].
       apply Hpre.
+      hnf; cbn; repeat constructor; auto.
+  Qed.
+
+  Record R_sys_putc_correct c k z m st st' ret := {
+    (* New itree is old k, or same as old itree if send failed *)
+    putc_z' := if 0 <=? Int.signed ret then k else z;
+
+    (* Post condition holds on new state, itree, and result *)
+    putc_post_ok : putchar_post m m ret (c, k) putc_z';
+    (* The itrees and OS traces agree on the external events *)
+    putc_itree_trace_ok : trace_itree_match z putc_z' st.(io_tx_log) st'.(io_tx_log);
+    (* The new trace is valid *)
+    (* TODO: have to define valid trace condition for putc *)
+    (* putc_trace_ok : valid_trace st'; *)
+  }.
+
+  Lemma sys_putc_correct c k z m st st' :
+    (* Initial trace is valid *)
+    valid_trace st ->
+    (* Pre condition holds *)
+    putchar_pre m (c, k) z ->
+    (* c is passed as an argument *)
+    get_sys_arg st = Vint c ->
+    (* sys_putc returns some state *)
+    sys_putc_spec st = Some st' ->
+    exists ret,
+      get_sys_ret st' = Vint ret /\
+      R_sys_putc_correct c k z m st st' ret.
+  Proof.
+    unfold putchar_pre, get_sys_arg, get_sys_ret; intros Hvalid Hpre Harg Hspec.
+    pose proof Hspec as Htrace_case.
+    unfold sys_putc_spec in Hspec; destruct_spec Hspec.
+    prename (thread_serial_putc_spec) into Hput.
+    apply thread_serial_putc_putc_trace_case in Hput.
+    assert (-1 <= z1 <= 255).
+    { pose proof (Z.mod_pos_bound z0 256 ltac:(lia)).
+      destruct Hput as (? & [(? & ?) | (? & ?)]); subst; lia.
+    }
+    unfold uctx_set_errno_spec in Hspec; destruct_spec Hspec.
+    prename (uctx_set_retval1_spec) into Hspec.
+    unfold uctx_set_retval1_spec in Hspec; destruct_spec Hspec.
+    prename (uctx_arg2_spec) into Hspec.
+    unfold uctx_arg2_spec in Hspec; destruct_spec Hspec.
+    destruct r1; cbn in *.
+    repeat (rewrite ZMap.gss in * || rewrite ZMap.gso in * by easy); subst; inj.
+    do 2 esplit; eauto.
+    eapply sys_putc_trace_case in Htrace_case; eauto.
+    2: unfold get_sys_ret; cbn; repeat (rewrite ZMap.gss || rewrite ZMap.gso by easy); auto.
+    constructor; eauto; hnf.
+    - (* putchar_post *)
+      split; auto; cbn in *.
+      rewrite Int.signed_repr by (cbn; lia).
+      destruct (Coqlib.zeq z1 (-1)); subst; auto.
+      destruct (eq_dec.eq_dec _ _); try easy.
+      rewrite Zle_imp_le_bool by lia.
+      destruct Hput as (? & [(? & ?) | (? & ?)]); subst; auto; lia.
+    - (* trace_itree_match *)
+      rewrite Int.signed_repr in * by (cbn; lia).
+      cbn in *; destruct Htrace_case as (Htr & Hcase).
+      intros * Htrace; cbn.
+      destruct Hcase as [(? & ->) | (? & Heq)]; subst; auto.
+      pose proof (Z.mod_pos_bound (Int.unsigned c) 256 ltac:(lia)).
+      rewrite Zle_imp_le_bool in Htrace by lia.
+      unshelve erewrite Heq; try solve [constructor].
+      eapply Traces.sutt_trace_incl; eauto; cbn.
+      rewrite Int.repr_unsigned.
       hnf; cbn; repeat constructor; auto.
   Qed.
 
